feels like we only go backwards

coq/two/IndistinguishabilityTwo.v
@@ -1,4 +1,4 @@
-Require Import Program.Tactics.
+Require Import Program.Tactics. 
 Require Import MyTactics.
 Require Import LabelAlgebra.
 Require Import LambdaTwoSyntax.
@@ -6,16 +6,14 @@ Require Import LambdaTwoSyntax.
 (** * Indistinguishability relations. *) 
 Section IndistinguishabilityTwo.
 
-Context (L : two)
-        (P : value -> value -> Prop)
-        (Prefl : forall x, P x x).
+Context (L : two) (P : nat -> Prop).
 
 Fixpoint atom_LPequiv a1 a2 : Prop :=
   match a1, a2 with
     | Atom v1 l1, Atom v2 l2 =>
       (L = Bottom2 /\ l1 = l2 /\ l1 = Top2 /\
        match v1, v2 with
-         | VNat n1, VNat n2 => P v1 v2
+         | VNat n1, VNat n2 => P n1 = P n2
          | VClos e1 t1, VClos e2 t2 => value_LPequiv v1 v2
          | _, _ => True
        end) \/
@@ -24,10 +22,11 @@ Fixpoint atom_LPequiv a1 a2 : Prop :=
   end
 with value_LPequiv v1 v2 : Prop :=
        match v1, v2 with
+         | VBool b1, VBool b2 => b1 = b2
          | VNat n1, VNat n2 => n1 = n2
          | VClos e1 t1, VClos e2 t2 =>
            list_forall2 atom_LPequiv e1 e2 /\ t1 = t2
-         | VNat _, _ | VClos _ _, _ => False
+         | VBool _, _ | VNat _, _ | VClos _ _, _ => False
        end.
 
 Definition env_LPequiv : env -> env -> Prop :=
@@ -47,27 +46,31 @@ Lemma atom_LPequiv_raise :
     atom_LPequiv (Atom v1 Top2) (Atom v2 Top2).
 Proof.
   intros v1 v2 H. destruct L.
-    destruct v1; destruct v2; destruct H; destruct H; destruct_conjs;
+  - destruct v1; destruct v2; destruct H; destruct H; destruct_conjs;
         inversion H; try inversion H1; subst; auto.
-      destruct H2. left. auto.
-      right. right. repeat (split; auto).
-      left. auto.
-      right. right. auto.
-    destruct v1; destruct v2; destruct H; destruct H; destruct_conjs;
-        inversion H; inversion H1; inversion H2.
-      left. repeat (split; auto). subst. auto. 
-      right. right. repeat (split; auto).
-      left. auto.
-      right. right. auto.
+    + destruct H2. left. auto.
+    + right. right. auto.
+    + left. auto.
+    + right. right. auto.
+    + left. auto.
+    + right. right. auto.
+  - destruct v1; destruct v2; destruct H; destruct H; destruct_conjs;
+        inversion H; inversion H1; inversion H2; subst.
+    + destruct H2. left. auto.
+    + right. right. auto.
+    + left. auto.
+    + right. right. auto.
+    + left. auto.
+    + right. right.  auto.
 Qed.
 
 End IndistinguishabilityTwo.
 
-Definition atom_Lequiv := fun L => atom_LPequiv L (fun _ _ => True).
+Definition atom_Lequiv := fun L => atom_LPequiv L (fun _ => True).
 
-Definition value_Lequiv := fun L => value_LPequiv L (fun _ _ => True).
+Definition value_Lequiv := fun L => value_LPequiv L (fun _ => True).
 
-Definition env_Lequiv := fun L => env_LPequiv L (fun _ _ => True).
+Definition env_Lequiv := fun L => env_LPequiv L (fun _ => True).
 
 Lemma atom_value_env_LPequiv_Lequiv :
   forall L P,
@@ -105,7 +108,9 @@ Proof.
           (destruct H; destruct H; destruct_conjs; try inversion H; auto).
       apply Hv in H0. right. right. auto.
   - intros n1 v2 H. destruct v2; inversion H; reflexivity.
-  - intros e1 He t1 v2 H. destruct v2 as [| e2 t2].
+  - intros n1 v2 H. destruct v2; inversion H; reflexivity.
+  - intros e1 He t1 v2 H. destruct v2 as [| | e2 t2].
+    + inversion H.
     + inversion H.
     + assert (env_LPequiv L P e1 e2) by (destruct H; auto).
       assert (t2 = t1) by (destruct H; symmetry; assumption).
@@ -131,62 +136,3 @@ Lemma env_LPequiv_Lequiv :
   forall L P e1 e2,
     env_LPequiv L P e1 e2 -> env_Lequiv L e1 e2.
 Proof. apply atom_value_env_LPequiv_Lequiv. Qed.
-
-Lemma atom_value_env_Top2equiv_Top2Pequiv :
-  forall P,
-    (forall a1 a2,
-       atom_Lequiv Top2 a1 a2 -> atom_LPequiv Top2 P a1 a2)
-    /\ (forall v1 v2,
-          value_Lequiv Top2 v1 v2 -> value_LPequiv Top2 P v1 v2)
-    /\ (forall e1 e2,
-          env_Lequiv Top2 e1 e2 -> env_LPequiv Top2 P e1 e2).
-Proof.
-  intros. apply atom_value_env_mutind.
-  - intros v1 Hv l1 a2 H. destruct a2 as [v2 l2].
-    assert (l2 = l1) by
-        (apply atom_LPequiv_lab_inv in H; subst; auto). 
-    assert (value_LPequiv Top2 P v1 v2) by
-        (apply Hv; destruct H; destruct H; destruct_conjs; inversion H; auto).
-    right. right. auto.
-  - intros n1 v2 H. destruct v2; destruct H; reflexivity.
-  - intros e1 He t1 v2 H. destruct v2 as [n2 | e2 t2]; destruct H; subst.
-    split; try apply He; auto.
-  - intros e1 Ha e2 H. generalize dependent e2.
-    induction e1 as [| a1 e1']; intros; destruct e2 as [| a2 e2']; auto.
-    split; destruct H.
-    + apply (Ha 0); auto.
-    + apply IHe1'; intros; try apply (Ha (S n)); auto.
-Qed.
-
-Lemma atom_Top2equiv_Top2Pequiv :
-  forall P a1 a2,
-    atom_Lequiv Top2 a1 a2 -> atom_LPequiv Top2 P a1 a2.
-Proof. apply atom_value_env_Top2equiv_Top2Pequiv. Qed.
-
-Lemma value_Top2equiv_Top2Pequiv :
-  forall P v1 v2,
-    value_Lequiv Top2 v1 v2 -> value_LPequiv Top2 P v1 v2.
-Proof. apply atom_value_env_Top2equiv_Top2Pequiv. Qed.
-
-Lemma env_Top2equiv_Top2Pequiv :
-  forall P e1 e2,
-    env_Lequiv Top2 e1 e2 -> env_LPequiv Top2 P e1 e2.
-Proof. apply atom_value_env_Top2equiv_Top2Pequiv. Qed.
-
-Lemma atom_Top2Pequiv_lower :
-  forall P v1 v2,
-    atom_LPequiv Top2 P (Atom v1 Top2) (Atom v2 Top2) ->
-    atom_LPequiv Top2 P (Atom v1 Bottom2) (Atom v2 Bottom2).
-Proof.
-  intros.
-  destruct v1 as [n1 | e1 t1]; destruct v2 as [n2 | e2 t2].
-  + destruct H; destruct H; destruct_conjs;
-    inversion H; subst; right; right; auto.
-  + destruct H; destruct H; destruct_conjs;
-    inversion H; inversion H1.
-  + destruct H; destruct H; destruct_conjs;
-    inversion H; inversion H1.
-  + destruct H; destruct H; destruct_conjs;
-    inversion H; subst; right; right; auto.
-Qed.
-  
