coq/two/LambdaTwo.v
@@ -1,55 +1,37 @@
-Require Import Arith. 
-Require Import Wf_nat.
-Require Import LibTactics.
-
 Require Export LambdaTwoSyntax.
 Require Export IndistinguishabilityTwo.
 
-Definition eval : nat -> two -> (value -> value -> Prop) ->
-                  two -> env -> term -> atom -> Prop.
-  refine
-    (Fix lt_wf (fun _ => two -> (value -> value -> Prop) ->
-                         two -> env -> term -> atom -> Prop)
-         (fun (k : nat)
-              (eval : forall k' : nat,
-                        k' < k -> two -> (value -> value -> Prop) ->
-                        two -> env -> term -> atom -> Prop) =>
-            fun (L : two) (P : value -> value -> Prop)
-                (pc : two) (e : env) (t : term) (a : atom) =>
-              match t with
-                | TNat n =>
-                  a = Atom (VNat n) pc
-                | TVar n =>
-                  exists v l,
-                    atIndex e n = Some (Atom v l) /\
-                    a = Atom v (l ⊔ pc)
-                | TAbs t' =>
-                  a = Atom (VClos e t') pc
-                | TApp t1 t2 =>
-                  exists k' e1' t1' l1 a2 a3,
-                    if lt_dec k' k then
-                      eval k' _ L P pc e t1 (Atom (VClos e1' t1') l1) /\
-                      eval k' _ L P pc e t2 a2 /\
-                      eval k' _ L P l1 (a2 :: e1') t1' a3 /\
-                      a = a3
-                    else False
-                | TDecl t1 t2 =>
-                  exists k' e1' t1' l1 a2 v3 l3,
-                    if lt_dec k' k then
-                      eval k' _ L P pc e t1 (Atom (VClos e1' t1) l1) /\
-                      eval k' _ L P pc e t2 a2 /\
-                      eval k' _ L P l1 (a2 :: e1') t1' (Atom v3 l3) /\
-                      match l3 with
-                        | Bottom2 =>
-                          a = Atom v3 Bottom2
-                        | Top2 =>
-                          (* TODO *)
-                          (*(forall a2' e2' v3',
-                             env_LPequiv L P (a2 :: e1') (a2' :: e2') ->
-                             eval k' _ L P l1 (a2' :: e2') t1' (Atom v3' Top2) ->
-                             value_LPequiv L P v3 v3') /\*)
-                          a = Atom v3 Bottom2
-                      end
-                    else False
-                   end)); auto.
-Defined.
+Reserved Notation "P , pc ; e ⊢ t ⇓ a" (at level 70).
+Inductive eval : (nat -> Prop) -> two -> env -> term -> atom -> Prop :=
+| E_Bool : forall P pc e b,
+(* ------------------------------------------------ *)
+    P, pc; e ⊢ TBool b ⇓ Atom (VBool b) pc
+| E_Nat : forall P pc e n,
+(* ------------------------------------------------ *)
+    P, pc; e ⊢ TNat n ⇓ Atom (VNat n) pc
+| E_Var : forall P pc e n v l,
+    atIndex e n = Some (Atom v l) ->
+(* ------------------------------------------------ *)
+    P, pc; e ⊢ TVar n ⇓ Atom v (l ⊔ pc)
+| E_Abs : forall P pc e t,
+(* ------------------------------------------------ *)
+    P, pc; e ⊢ TAbs t ⇓ Atom (VClos e t) pc
+| E_App : forall P pc e t1 t2 e1' t1' l1 a2 a3,
+    P, pc; e ⊢ t1 ⇓ Atom (VClos e1' t1') l1 ->
+    P, pc; e ⊢ t2 ⇓ a2 ->
+    P, l1; a2 :: e1' ⊢ t1' ⇓ a3 ->
+(* ------------------------------------------------ *)
+    P, pc; e ⊢ TApp t1 t2 ⇓ a3
+| E_Decl1 : forall P pc e t n L,
+    P, pc; e ⊢ t ⇓ Atom (VNat n) L ->
+    P n ->
+(* ------------------------------------------------ *)
+    P, pc; e ⊢ TDecl t ⇓ Atom (VBool true) Bottom2
+| E_Decl2 : forall P pc e t n L,
+    P, pc; e ⊢ t ⇓ Atom (VNat n) L ->
+    ~ P n ->
+(* ------------------------------------------------ *)
+    P, pc; e ⊢ TDecl t ⇓ Atom (VBool false) Bottom2
+where "P , pc ; e ⊢ t ⇓ a" := (eval P pc e t a).
+
+Hint Constructors eval.
