coq/two/LambdaTwoNI.v
@@ -5,107 +5,111 @@ Require Import LibTactics.
 Section NI.
 
 Theorem non_interference_strong_observer :
-  forall L P k pc e1 e2 t a1 a2,
+  forall L P pc e1 e2 t a1 a2,
     env_LPequiv L P e1 e2 ->
-    eval L P pc e1 t k a1 -> 
-    eval L P pc e2 t k a2 -> 
-    (forall x, P x x) ->
+    P, pc; e1 ⊢ t ⇓ a1 ->
+    P, pc; e2 ⊢ t ⇓ a2 ->
     atom_LPequiv L P a1 a2.
 Proof.
-  introv He Heval1 Heval2 Prefl.
-  gen pc e1 e2 t a1 a2.
-  induction k as [| k']; intros; destruct t; auto.
+  introv He Heval1 Heval2; gen e2 a2.
+  induction Heval1; intros; rename e into e1.
+  - (* E_Bool *)
+    inversion Heval2; subst.
+    destruct L; destruct pc.
+    + right. left. auto.
+    + left. auto.
+    + right. right. auto.
+    + right. right. auto.
   - (* E_Nat *)
-    simpl in Heval1; simpl in Heval2; subst.
+    inversion Heval2; subst.
     destruct L; destruct pc.
     + right. left. auto.
     + left. auto.
     + right. right. auto.
     + right. right. auto.
   - (* E_Var *)
-    simpl in Heval1; simpl in Heval2; subst.
-    destruct Heval1 as [v1 [l1 [H1 H2]]].
-    destruct Heval2 as [v2 [l2 [H1' H2']]].
+    inversion Heval2; subst;
+    rename v into v1; rename l into l1;
+    rename v0 into v2; rename l0 into l2.
     assert (Ha: atom_LPequiv L P (Atom v1 l1) (Atom v2 l2)) by
         (eapply list_forall2_atIndex; eauto).
-    assert (l2 = l1) by
-        (apply atom_LPequiv_lab_inv in Ha; auto).
-    destruct pc; destruct l1; subst; auto;
-    apply atom_LPequiv_raise; assumption.
+    assert (l2 = l1) by (apply atom_LPequiv_lab_inv in Ha; auto); subst.
+    destruct pc.
+    + rewrite join_bot. assumption.
+    + rewrite join_top. destruct l1; try assumption.
+      apply atom_LPequiv_raise. assumption.
   - (* E_Abs *)
-    simpl in Heval1; simpl in Heval2; subst.
+    inversion Heval2; subst.
     destruct L; destruct pc.
     + right. left. auto.
     + left. auto.
     + right. right. auto.
     + right. right. auto.
   - (* E_App *)
-    rename a1 into a; rename a2 into a'.
-    rename e1 into e; rename e2 into e'.
-    simpl in Heval1; simpl in Heval2.
-    destruct Heval1 as
-        [e1' [t1' [l1 [a2 [a3 [H1 [H2 [H3 Ha]]]]]]]].
-    destruct Heval2 as
-        [e2' [t2' [l2 [a2' [a3' [H1' [H2' [H3' Ha']]]]]]]].
-    remember (Atom (VClos e1' t1') l1) as a1.
-    remember (Atom (VClos e2' t2') l2) as a1'.
-    assert (IH1: atom_LPequiv L P a1 a1') by
-        (eapply IHk'; eauto).
-    assert (l2 = l1) by
-        (subst; apply atom_LPequiv_lab_inv in IH1; auto).
-    assert (t2' = t1' /\ env_LPequiv L P e1' e2') by
-        (split; subst; destruct IH1 as [H |];
-         destruct H; destruct_conjs; auto).
-    destruct_conjs; subst.
-    assert (IH2: atom_LPequiv L P a2 a2') by
-        (apply (IHk' pc e e' He t2); auto).
-    assert (env_LPequiv L P (a2 :: e1') (a2' :: e2')) by
-        (split; auto).
-    eapply IHk'; eauto.
-  - (* E_Decl *)
-    rename a1 into a; rename a2 into a'.
-    rename e1 into e; rename e2 into e'.
-    simpl in Heval1; simpl in Heval2.
-    destruct Heval1 as
-        [e1' [t1' [l1 [a2 [v3 [l3 [H1 [H2 [H3 H4]]]]]]]]].
-    destruct Heval2 as
-        [e2' [t2' [l2 [a2' [v3' [l3' [H1' [H2' [H3' H4']]]]]]]]].
-    remember (Atom (VClos e1' t1') l1) as a1.
-    remember (Atom (VClos e2' t2') l2) as a1'.
-    assert (IH1: atom_LPequiv L P a1 a1') by
-        (eapply IHk'; eauto).
-    assert (l2 = l1) by
-        (subst; apply atom_LPequiv_lab_inv in IH1; auto).
-    assert (t2' = t1' /\ env_LPequiv L P e1' e2') by
-        (split; subst; destruct IH1 as [H |];
-         destruct H; destruct_conjs; auto).
-    destruct_conjs; subst.
-    assert (IH2: atom_LPequiv L P a2 a2') by
-        (apply (IHk' pc e e' He t2); auto).
-    assert (env_LPequiv L P (a2 :: e1') (a2' :: e2')) by
-        (split; auto).
-    assert (IH3: atom_LPequiv L P (Atom v3 l3) (Atom v3' l3')) by
-        (eapply IHk'; eauto).
-    assert (l3' = l3) by
-        (apply atom_LPequiv_lab_inv in IH3; auto); subst.
-    destruct l3; subst; auto.
-    destruct_conjs; subst.
-    assert (value_LPequiv L P v3 v3') by
-        (eapply H4; eauto).
-    destruct L.
-    + right. left. auto.
-    + right. right. auto.
+    inversion Heval2; subst;
+    rename e1'0 into e1''; rename t1'0 into t1''; rename l0 into l1';
+    rename a1 into a2'; rename a0 into a3';
+    rename H1 into Heval2_1; rename H5 into Heval2_2; rename H7 into Heval2_3.
+    remember (Atom (VClos e1' t1') l1) as a1;
+    remember (Atom (VClos e1'' t1'') l1') as a1'.
+    assert (Ha1: atom_LPequiv L P a1 a1') by (eapply IHHeval1_1; eauto); subst.
+    assert (Ha2: atom_LPequiv L P a2 a2') by (eapply IHHeval1_2; eauto).
+    assert (l1' = l1) by (apply atom_LPequiv_lab_inv in Ha1; auto); subst.
+    assert (He1: t1'' = t1' /\ env_LPequiv L P e1' e1'') by
+        (split; destruct Ha1; destruct H; destruct_conjs; subst; auto);
+      destruct He1 as [Ht He1]; subst.
+    assert (He': env_LPequiv L P (a2 :: e1') (a2' :: e1'')) by (split; auto).
+    eapply IHHeval1_3; eauto.
+  - (* E_Decl1 *)
+    inversion Heval2; subst;
+    rename n into n1; rename L0 into l1;
+    rename n0 into n2; rename L1 into l2.
+    + destruct L; right.
+      * left. auto.
+      * right. auto.
+    + assert (Ha: atom_LPequiv L P (Atom (VNat n1) l1) (Atom (VNat n2) l2)) by
+          (eapply IHHeval1; eauto).
+      assert (l2 = l1) by (apply atom_LPequiv_lab_inv in Ha; auto); subst.
+      destruct L;
+        (destruct l1;
+         try (assert (~ P n1) by
+                 (destruct Ha; destruct H0; destruct_conjs;
+                  inversion H3; subst; auto));
+         try (assert (P n2) by
+                 (destruct Ha; destruct H0; destruct_conjs; 
+                  try rewrite <- H4; subst; auto));
+         contradiction).
+  - (* E_Decl2 *)
+    inversion Heval2; subst;
+    rename n into n1; rename L0 into l1;
+    rename n0 into n2; rename L1 into l2;
+    assert (Ha: atom_LPequiv L P (Atom (VNat n1) l1) (Atom (VNat n2) l2)) by
+        (eapply IHHeval1; eauto);
+    assert (l2 = l1) by (apply atom_LPequiv_lab_inv in Ha; auto); subst.
+    + destruct L;
+      (destruct l1;
+       try (assert (P n1) by
+               (destruct Ha; destruct H0; destruct_conjs;
+                inversion H3; subst; auto));
+       try (assert (P n1) by
+               (destruct Ha; destruct H0; destruct_conjs;
+                try rewrite H4; subst; auto));
+       contradiction).
+    + destruct L; destruct l1; right.
+      * left. auto.
+      * left. auto.
+      * right. auto.
+      * right. auto.
 Qed.
 
 Theorem non_interference :
-  forall L (P : value -> value -> Prop) k pc e1 e2 t a1 a2,
-    (forall x, P x x) ->
+  forall L (P : nat -> Prop) pc e1 e2 t a1 a2,
     env_LPequiv L P e1 e2 ->
-    eval L P pc e1 t k a1 ->
-    eval L P pc e2 t k a2 ->
+    P, pc; e1 ⊢ t ⇓ a1 ->
+    P, pc; e2 ⊢ t ⇓ a2 ->
     atom_Lequiv L a1 a2.
 Proof.
-  intros L P k pc e1 e2 t a1 a2 Prefl He Heval1 Heval2.
+  intros L P pc e1 e2 t a1 a2 He Heval1 Heval2.
   eapply non_interference_strong_observer in Heval2; eauto.
   eapply atom_LPequiv_Lequiv. eassumption.
 Qed.
